wip

theories/map_to_multiset.v
@@ -3,17 +3,30 @@ From diris Require Export rtypesystem.
 
 Definition list_to_multiset {A} (l : list A) := MultiSet l.
 
+Lemma list_to_multiset_cons {A:ofe} (l : list A) (x : A) :
+  list_to_multiset (x :: l) ≡ {[ x ]} ⋅ list_to_multiset l.
+Proof. done. Qed.
+
 Instance list_to_multiset_proper {A:ofe} : Proper ((≡ₚ) ==> (≡)) (list_to_multiset (A:=A)).
 Proof.
-Admitted.
+  intros ???.
+  induction H; eauto.
+  - rewrite !list_to_multiset_cons IHPermutation //.
+  - rewrite !list_to_multiset_cons !assoc (comm (⋅) {[y]}) //.
+  - by rewrite IHPermutation1.
+Qed.
 
 Section map_to_multiset.
-  Implicit Type m : gmap bool chan_type.
-  Implicit Type x : multiset clabel.
-  Implicit Type i : bool.
-  Implicit Type v : chan_type.
+  Context {K : ofe}.
+  Context `{HC : Countable K}.
+  Context {HL : LeibnizEquiv K}.
+  Context {A:ofe}.
+  Implicit Type m : gmap K A.
+  Implicit Type x : multiset (K*A).
+  Implicit Type i : K.
+  Implicit Type v : A.
 
-  Definition map_to_multiset m : multiset clabel :=
+  Definition map_to_multiset m :=
     list_to_multiset (map_to_list m).
 
   Lemma map_to_multiset_empty :
@@ -27,20 +40,10 @@ Section map_to_multiset.
     (∀ i, m !! i = None) ->
     map_to_multiset m = ε.
   Proof.
-    intros H.
+    intros HH.
     assert (m = ∅) as -> by by apply map_empty.
     apply map_to_multiset_empty.
   Qed.
-
-  Lemma map_to_multiset_lookup m i v x :
-    {[ (i, v) ]} ⋅ x ≡ map_to_multiset m ->
-    m !! i = Some v.
-  Proof.
-    intros H.
-    unfold map_to_multiset in H.
-    symmetry in H.
-    (* apply map_to_list_insert_inv in H. *)
-  Admitted.
 
   Lemma map_to_multiset_insert m i v :
     m !! i = None ->
@@ -51,18 +54,55 @@ Section map_to_multiset.
     rewrite map_to_list_insert //.
   Qed.
 
+  Lemma map_to_multiset_lookup m i v x :
+    {[ (i, v) ]} ⋅ x ≡ map_to_multiset m ->
+    m !! i ≡ Some v.
+  Proof.
+    revert x. induction m using map_ind; intros x'.
+    - rewrite map_to_multiset_empty.
+      intros HH. eapply multiset_empty_mult in HH as [].
+      exfalso.
+      eapply multiset_empty_neq_singleton; done.
+    - rewrite map_to_multiset_insert //.
+      intros HH.
+      eapply mset_xsplit in HH as (e11 & e12 & e21 & e22 & Q1 & Q2 & Q3 & Q4).
+      eapply multiset_singleton_mult in Q1.
+      eapply multiset_singleton_mult in Q3.
+      destruct Q1 as [[H11 H12]|[H11 H12]].
+      + rewrite ->H12 in Q4.
+        symmetry in Q4.
+        pose proof (IHm _ Q4) as H6.
+        rewrite lookup_insert_spec.
+        case_decide; subst; eauto.
+        rewrite H in H6. inversion H6.
+      + rewrite ->H12 in Q4.
+        revert Q4. rewrite left_id. intros Q4.
+        destruct Q3 as [[H31 H32]|[H31 H32]].
+        * rewrite ->H11 in H31.
+          exfalso. eapply multiset_empty_neq_singleton, multiset_empty_equiv; done.
+        * rewrite ->H11 in H31.
+          eapply inj in H31; last apply _.
+          inversion H31; simpl in *.
+          rewrite H1.
+          assert (i = i0).
+          { apply leibniz_equiv. done. } subst.
+          rewrite lookup_insert //.
+  Qed.
+
   Lemma map_to_multiset_delete m i v x :
     {[ (i, v) ]} ⋅ x ≡ map_to_multiset m ->
     x ≡ map_to_multiset (delete i m).
   Proof.
-    intros H.
-    pose proof (map_to_multiset_lookup _ _ _ _ H) as Hi.
-    replace m with (<[ i := v ]> (delete i m)) in H; last first.
+    intros HH.
+    pose proof (map_to_multiset_lookup _ _ _ _ HH) as Hi.
+    inversion Hi; subst.
+    replace m with (<[ i := x0 ]> (delete i m)) in HH; last first.
     { apply map_eq. intros j.
       rewrite lookup_insert_spec lookup_delete_spec.
-      case_decide; naive_solver. }
-    rewrite ->map_to_multiset_insert in H; last apply lookup_delete.
-    by apply multiset_mult_singleton_inv in H.
+      case_decide; subst; eauto. }
+    rewrite ->map_to_multiset_insert in HH; last apply lookup_delete.
+    rewrite ->H1 in HH.
+    by apply multiset_mult_singleton_inv in HH.
   Qed.
 
   Lemma map_to_multiset_update m x i v v' :
